src/ExampleScript.sml
@@ -201,6 +201,17 @@ in
 				(combine (["ex_A1", "ex_A2", "ex_A3"], nodes))
 end;
 
+val (WB_rules, WB_coind, WB_cases) = Hol_coreln `
+    (!(P :('a, 'b) CCS) (Q :('a, 'b) CCS).
+       (!l.
+	 (!P'. TRANS P  (label l) P' ==>
+	       (?Q'. WEAK_TRANS Q (label l) Q' /\ WB P' Q')) /\
+	 (!Q'. TRANS Q (label l) Q' ==>
+	       (?P'. WEAK_TRANS P  (label l) P' /\ WB P' Q'))) /\
+       (!P'. TRANS P tau P' ==> (?Q'. EPS Q Q' /\ WB P' Q')) /\
+       (!Q'. TRANS Q tau Q' ==> (?P'. EPS P P' /\ WB P' Q'))
+      ==> WB P Q)`;
+
 val _ = export_theory ();
 val _ = html_theory "Example";
 
